Add iris/base_logic/lib/semiauth_twins.

theories/iris/base_logic/lib/auth_twins.v
@@ -3,24 +3,18 @@ From zebre Require Import
 From zebre.iris.base_logic Require Export
   lib.base.
 From zebre.iris.base_logic Require Import
-  lib.ghost_var
-  lib.auth_mono
-  lib.twins.
+  lib.semiauth_twins.
 From zebre.iris Require Import
   diaframe.
 From zebre Require Import
   options.
 
 Class AuthTwinsG Σ {A : ofe} (R : relation A) := {
-  #[local] auth_twins_G_var_G :: GhostVarG Σ (gname * gname) ;
-  #[local] auth_twins_G_mono_G :: AuthMonoG Σ R ;
-  #[local] auth_twins_G_twins_G :: TwinsG Σ A ;
+  #[local] auth_twins_G_semiauth_twins_G :: SemiauthTwinsG Σ R unitO ;
 }.
 
 Definition auth_twins_Σ {A : ofe} (R : relation A) := #[
-  ghost_var_Σ (gname * gname) ;
-  auth_mono_Σ R ;
-  twins_Σ A
+  semiauth_twins_Σ R unitO
 ].
 #[global] Instance subG_auth_twins_Σ Σ {A : ofe} (R : relation A) :
   subG (auth_twins_Σ R) Σ →
@@ -38,20 +32,24 @@ Section auth_twins_G.
 
   Implicit Types a b : A.
 
+  Definition auth_twins_name :=
+    semiauth_twins_name.
+  Implicit Types γ : auth_twins_name.
+
+  #[global] Instance auth_twins_name_eq_dec : EqDecision auth_twins_name :=
+    ltac:(solve_decision).
+  #[global] Instance auth_twins_name_countable :
+    Countable auth_twins_name.
+  Proof.
+    apply _.
+  Qed.
+
   Definition auth_twins_auth γ a : iProp Σ :=
-    ∃ γs,
-    ghost_var γ (DfracOwn (1/3)) γs ∗
-    auth_mono_auth R γs.1 (DfracOwn 1) a.
+    semiauth_twins_auth R unitO γ a.
   Definition auth_twins_twin1 γ a : iProp Σ :=
-    ∃ γs,
-    ghost_var γ (DfracOwn (1/3)) γs ∗
-    auth_mono_lb R γs.1 a ∗
-    twins_twin1 γs.2 (DfracOwn 1) a.
+    semiauth_twins_twin1 R unitO γ a ().
   Definition auth_twins_twin2 γ a : iProp Σ :=
-    ∃ γs,
-    ghost_var γ (DfracOwn (1/3)) γs ∗
-    auth_mono_lb R γs.1 a ∗
-    twins_twin2 γs.2 a.
+    semiauth_twins_twin2 R unitO γ a ().
 
   #[global] Instance auth_twins_auth_timeless γ a :
     Timeless (auth_twins_auth γ a).
@@ -78,13 +76,7 @@ Section auth_twins_G.
       auth_twins_twin1 γ a ∗
       auth_twins_twin2 γ a.
   Proof.
-    iMod (auth_mono_alloc _ a) as "(%γ_mono & Hauth)".
-    iDestruct (auth_mono_lb_get with "Hauth") as "#Hlb".
-    iMod (twins_alloc' (twins_G := auth_twins_G_twins_G) a) as "(%γ_twins & Htwin1 & Htwin2)".
-    iMod (ghost_var_alloc (γ_mono, γ_twins)) as "(%γ & Hγ)".
-    iEval (assert (1 = 1/3 + (1/3 + 1/3))%Qp as -> by compute_done) in "Hγ".
-    iDestruct "Hγ" as "(Hγ1 & (Hγ2 & Hγ3))".
-    iSteps.
+    apply semiauth_twins_alloc.
   Qed.
 
   Lemma auth_twins_auth_exclusive `{!AntiSymm (≡) Rs} γ a1 a2 :
@@ -92,18 +84,14 @@ Section auth_twins_G.
     auth_twins_auth γ a2 -∗
     False.
   Proof.
-    iIntros "(%γs & Hγ1 & Hauth1) (%_γs & Hγ2 & Hauth2)".
-    iDestruct (ghost_var_agree with "Hγ1 Hγ2") as %<-.
-    iApply (auth_mono_auth_exclusive with "Hauth1 Hauth2").
+    apply: semiauth_twins_auth_exclusive.
   Qed.
   Lemma auth_twins_auth_exclusive_L `{!LeibnizEquiv A} `{!AntiSymm (=) Rs} γ a1 a2 :
     auth_twins_auth γ a1 -∗
     auth_twins_auth γ a2 -∗
     False.
   Proof.
-    iIntros "(%γs & Hγ1 & Hauth1) (%_γs & Hγ2 & Hauth2)".
-    iDestruct (ghost_var_agree with "Hγ1 Hγ2") as %<-.
-    iApply (auth_mono_auth_exclusive_L with "Hauth1 Hauth2").
+    apply: semiauth_twins_auth_exclusive_L.
   Qed.
 
   Lemma auth_twins_twin1_exclusive γ a1 a2 :
@@ -111,9 +99,7 @@ Section auth_twins_G.
     auth_twins_twin1 γ a2 -∗
     False.
   Proof.
-    iIntros "(%γs & Hγ1 & _ & Htwin1_1) (%_γs & Hγ2 & _ & Htwin1_2)".
-    iDestruct (ghost_var_agree with "Hγ1 Hγ2") as %<-.
-    iApply (twins_twin1_exclusive with "Htwin1_1 Htwin1_2").
+    apply semiauth_twins_twin1_exclusive.
   Qed.
 
   Lemma auth_twins_twin2_exclusive γ a1 a2 :
@@ -121,9 +107,7 @@ Section auth_twins_G.
     auth_twins_twin2 γ a2 -∗
     False.
   Proof.
-    iIntros "(%γs & Hγ1 & _ & Htwin2_1) (%_γs & Hγ2 & _ & Htwin2_2)".
-    iDestruct (ghost_var_agree with "Hγ1 Hγ2") as %<-.
-    iApply (twins_twin2_exclusive with "Htwin2_1 Htwin2_2").
+    apply semiauth_twins_twin2_exclusive.
   Qed.
 
   Lemma auth_twins_valid_1 γ a b :
@@ -131,18 +115,14 @@ Section auth_twins_G.
     auth_twins_twin1 γ b -∗
     ⌜Rs b a⌝.
   Proof.
-    iIntros "(%γs & Hγ1 & Hauth) (%_γs & Hγ2 & Hlb & _)".
-    iDestruct (ghost_var_agree with "Hγ1 Hγ2") as %<-.
-    iApply (auth_mono_lb_valid with "Hauth Hlb").
+    apply semiauth_twins_valid_1.
   Qed.
   Lemma auth_twins_valid_2 γ a b :
     auth_twins_auth γ a -∗
     auth_twins_twin2 γ b -∗
     ⌜Rs b a⌝.
   Proof.
-    iIntros "(%γs & Hγ1 & Hauth) (%_γs & Hγ2 & Hlb & _)".
-    iDestruct (ghost_var_agree with "Hγ1 Hγ2") as %<-.
-    iApply (auth_mono_lb_valid with "Hauth Hlb").
+    apply semiauth_twins_valid_2.
   Qed.
 
   Lemma auth_twins_agree γ a1 a2 :
@@ -150,27 +130,24 @@ Section auth_twins_G.
     auth_twins_twin2 γ a2 -∗
     a1 ≡ a2.
   Proof.
-    iIntros "(%γs & Hγ1 & _ & Htwin1) (%_γs & Hγ2 & _ & Htwin2)".
-    iDestruct (ghost_var_agree with "Hγ1 Hγ2") as %<-.
-    iApply (twins_agree with "Htwin1 Htwin2").
+    iIntros "Htwin1 Htwin2".
+    iDestruct (semiauth_twins_agree with "Htwin1 Htwin2") as "($ & _)".
   Qed.
   Lemma auth_twins_agree_discrete `{!OfeDiscrete A} γ a1 a2 :
     auth_twins_twin1 γ a1 -∗
     auth_twins_twin2 γ a2 -∗
     ⌜a1 ≡ a2⌝.
   Proof.
-    iIntros "(%γs & Hγ1 & _ & Htwin1) (%_γs & Hγ2 & _ & Htwin2)".
-    iDestruct (ghost_var_agree with "Hγ1 Hγ2") as %<-.
-    iApply (twins_agree_discrete with "Htwin1 Htwin2").
+    iIntros "Htwin1 Htwin2".
+    iDestruct (semiauth_twins_agree_discrete with "Htwin1 Htwin2") as "($ & _)".
   Qed.
   Lemma auth_twins_agree_L `{!OfeDiscrete A} `{!LeibnizEquiv A} γ a1 a2 :
     auth_twins_twin1 γ a1 -∗
     auth_twins_twin2 γ a2 -∗
     ⌜a1 = a2⌝.
   Proof.
-    iIntros "(%γs & Hγ1 & _ & Htwin1) (%_γs & Hγ2 & _ & Htwin2)".
-    iDestruct (ghost_var_agree with "Hγ1 Hγ2") as %<-.
-    iApply (twins_agree_L with "Htwin1 Htwin2").
+    iIntros "Htwin1 Htwin2".
+    iDestruct (semiauth_twins_agree_L with "Htwin1 Htwin2") as "($ & _)".
   Qed.
 
   Lemma auth_twins_update_auth {γ a b1 b2} a' :
@@ -181,17 +158,7 @@ Section auth_twins_G.
       auth_twins_twin1 γ a' ∗
       auth_twins_twin2 γ a'.
   Proof.
-    assert (1 = 1/3 + (1/3 + 1/3))%Qp as Heq by compute_done.
-    iIntros "(%γs & Hγ1 & _) (%_γs & Hγ2 & _ & Htwin1) (%__γs & Hγ3 & _ & Htwin2)".
-    iDestruct (ghost_var_agree with "Hγ1 Hγ2") as %<-.
-    iDestruct (ghost_var_agree with "Hγ1 Hγ3") as %<-.
-    iCombine "Hγ1 Hγ2 Hγ3" as "Hγ". rewrite -Heq.
-    iMod (twins_update' (twins_G := auth_twins_G_twins_G) a' with "Htwin1 Htwin2") as "(Htwin1 & Htwin2)".
-    iMod (auth_mono_alloc _ a') as "(%γ_mono & Hauth)".
-    iDestruct (auth_mono_lb_get with "Hauth") as "#Hlb".
-    iMod (ghost_var_update (γ_mono, γs.2) with "Hγ") as "Hγ".
-    iEval (rewrite Heq) in "Hγ". iDestruct "Hγ" as "(Hγ1 & (Hγ2 & Hγ3))".
-    iSteps.
+    apply semiauth_twins_update_auth.
   Qed.
   Lemma auth_twins_update_twins {γ a1 a2} a :
     Rs a a1 →
@@ -201,12 +168,7 @@ Section auth_twins_G.
       auth_twins_twin1 γ a ∗
       auth_twins_twin2 γ a.
   Proof.
-    iIntros "%Ha1 %Ha2 (%γs & Hγ1 & #Hlb1 & Htwin1) (%_γs & Hγ2 & #Hlb2 & Htwin2)".
-    iDestruct (ghost_var_agree with "Hγ1 Hγ2") as %<-.
-    iMod (twins_update' (twins_G := auth_twins_G_twins_G) a with "Htwin1 Htwin2") as "(Htwin1 & Htwin2)".
-    iDestruct (auth_mono_lb_mono with "Hlb1") as "#Hlb1'"; first done.
-    iDestruct (auth_mono_lb_mono with "Hlb2") as "#Hlb2'"; first done.
-    iSteps.
+    apply semiauth_twins_update_twins.
   Qed.
   Lemma auth_twins_update_twins_L `{!OfeDiscrete A} `{!LeibnizEquiv A} {γ a1 a2} a :
     Rs a a1 →
@@ -215,15 +177,11 @@ Section auth_twins_G.
       auth_twins_twin1 γ a ∗
       auth_twins_twin2 γ a.
   Proof.
-    iIntros "%Ha (%γs & Hγ1 & #Hlb & Htwin1) (%_γs & Hγ2 & _ & Htwin2)".
-    iDestruct (ghost_var_agree with "Hγ1 Hγ2") as %<-.
-    iDestruct (twins_agree_L with "Htwin1 Htwin2") as %<-.
-    iMod (twins_update' (twins_G := auth_twins_G_twins_G) a with "Htwin1 Htwin2") as "(Htwin1 & Htwin2)".
-    iDestruct (auth_mono_lb_mono with "Hlb") as "#Hlb'"; first done.
-    iSteps.
+    apply: semiauth_twins_update_twins_L.
   Qed.
 End auth_twins_G.
 
+#[global] Opaque auth_twins_name.
 #[global] Opaque auth_twins_auth.
 #[global] Opaque auth_twins_twin1.
 #[global] Opaque auth_twins_twin2.
